proofs/fstar/extraction/Libcrux.Kem.Kyber.Kyber768.fsti
@@ -83,7 +83,7 @@ val encapsulate_768_
       Prims.l_True
       (fun _ -> Prims.l_True)
 
-val validate_public_key_768_ (public_key: Libcrux.Kem.Kyber.Types.t_KyberPublicKey (sz 1184))
+val validate_public_key_768_ (public_key: Libcrux.Kem.Kyber.Types.t_MlKemPublicKey (sz 1184))
     : Prims.Pure bool Prims.l_True (fun _ -> Prims.l_True)
 
 val generate_key_pair_768_ (randomness: t_Array u8 (sz 64))
